theories/Refinement/OSRefinementTheorem.v
@@ -1,0 +1,307 @@
+From Stdlib Require Import List.
+From RocqSched Require Import Foundation.Base.
+From RocqSched Require Import Semantics.Schedule.
+From RocqSched Require Import Abstractions.Scheduler.Interface.
+From RocqSched Require Import Abstractions.SchedulingAlgorithm.SchedulerBridge.
+From RocqSched Require Import Abstractions.SchedulingAlgorithm.TopMInterface.
+From RocqSched Require Import Abstractions.SchedulingAlgorithm.TopMSchedulerBridge.
+From RocqSched Require Import Multicore.Common.MultiCoreBase.
+From RocqSched Require Import Multicore.Common.Admissibility.
+From RocqSched Require Import Multicore.Common.PlacementFacts.
+From RocqSched Require Import Multicore.Common.ValidityFacts.
+From RocqSched Require Import Operational.Common.OSProjectionInterface.
+From RocqSched Require Import Operational.Common.ConcreteExecution.
+From RocqSched Require Import Operational.Common.LabeledExecution.
+From RocqSched Require Import Operational.Common.DelayModel.
+From RocqSched Require Import Operational.Common.DelayBudget.
+From RocqSched Require Import Operational.Common.Projection.
+From RocqSched Require Import Operational.Common.ProjectionLemmas.
+From RocqSched Require Import Operational.Common.ProjectionMulticoreValidity.
+From RocqSched Require Import Operational.Common.OSAdapterContract.
+From RocqSched Require Import Refinement.BoundedDelayRefinement.
+Import ListNotations.
+
+Lemma labeled_concrete_projection_sound_to_labeled_execution :
+  forall CState (P : OSLabeledProjection CState) jobs m
+         (ex : labeled_concrete_execution P m),
+    labeled_concrete_projection_sound jobs m ex ->
+    labeled_execution_projection_sound jobs m (concrete_to_labeled_execution ex).
+Proof.
+  intros CState P jobs m ex Hsound.
+  constructor.
+  - intros t c j Hlt Hrun.
+    exact (lcps_release_sound Hsound t c j Hlt Hrun).
+  - intros t c j Hlt Hrun.
+    exact (lcps_completion_sound Hsound t c j Hlt Hrun).
+Qed.
+
+Lemma labeled_concrete_projection_sound_implies_valid_schedule :
+  forall CState (P : OSLabeledProjection CState) jobs m
+         (ex : labeled_concrete_execution P m),
+    labeled_concrete_projection_sound jobs m ex ->
+    valid_schedule
+      jobs
+      m
+      (project_schedule (lex_trace (concrete_to_labeled_execution ex))).
+Proof.
+  intros CState P jobs m ex Hsound.
+  apply labeled_execution_projection_sound_implies_valid_schedule.
+  apply labeled_concrete_projection_sound_to_labeled_execution.
+  exact Hsound.
+Qed.
+
+Lemma labeled_concrete_multicore_projection_sound_to_labeled_execution :
+  forall CState (P : OSLabeledProjection CState) jobs adm m
+         (ex : labeled_concrete_execution P m),
+    labeled_concrete_multicore_projection_sound jobs adm m ex ->
+    labeled_execution_multicore_projection_sound
+      jobs adm m (concrete_to_labeled_execution ex).
+Proof.
+  intros CState P jobs adm m ex Hsound.
+  constructor.
+  - apply labeled_concrete_projection_sound_to_labeled_execution.
+    exact (lcmps_projection_sound Hsound).
+  - intros t.
+    exact (lcmps_idle_outside Hsound t).
+  - intros t.
+    exact (lcmps_placement Hsound t).
+Qed.
+
+Lemma labeled_concrete_multicore_projection_sound_implies_valid_schedule :
+  forall CState (P : OSLabeledProjection CState) jobs adm m
+         (ex : labeled_concrete_execution P m),
+    labeled_concrete_multicore_projection_sound jobs adm m ex ->
+    valid_schedule
+      jobs
+      m
+      (project_schedule (lex_trace (concrete_to_labeled_execution ex))).
+Proof.
+  intros CState P jobs adm m ex Hsound.
+  apply labeled_concrete_projection_sound_implies_valid_schedule.
+  exact (lcmps_projection_sound Hsound).
+Qed.
+
+Lemma labeled_concrete_multicore_projection_sound_implies_semantic_validity :
+  forall CState (P : OSLabeledProjection CState) jobs adm m
+         (ex : labeled_concrete_execution P m),
+    labeled_concrete_multicore_projection_sound jobs adm m ex ->
+    multicore_semantic_validity
+      jobs
+      m
+      (project_schedule (lex_trace (concrete_to_labeled_execution ex))).
+Proof.
+  intros CState P jobs adm m ex Hsound.
+  apply labeled_execution_multicore_projection_sound_implies_semantic_validity
+    with (adm := adm).
+  apply labeled_concrete_multicore_projection_sound_to_labeled_execution.
+  exact Hsound.
+Qed.
+
+Lemma labeled_concrete_multicore_projection_sound_implies_placement :
+  forall CState (P : OSLabeledProjection CState) jobs adm m
+         (ex : labeled_concrete_execution P m),
+    labeled_concrete_multicore_projection_sound jobs adm m ex ->
+    schedule_respects_admissibility
+      adm
+      m
+      (project_schedule (lex_trace (concrete_to_labeled_execution ex))).
+Proof.
+  intros CState P jobs adm m ex Hsound.
+  apply labeled_execution_multicore_projection_sound_implies_placement
+    with (jobs := jobs).
+  apply labeled_concrete_multicore_projection_sound_to_labeled_execution.
+  exact Hsound.
+Qed.
+
+Record os_delay_adapter_contract
+    {CState : Type}
+    (P : OSLabeledProjection CState)
+    (jobs : JobId -> Job)
+    (adm : admissible_cpu)
+    (m : nat) : Type :=
+  mkOSDelayAdapterContract {
+    odac_base : os_multicore_adapter_contract P jobs adm m;
+    odac_ideal_schedule : Schedule;
+    odac_delay_bounds : op_delay_bounds;
+    odac_delay_sources : DelayTrace;
+    odac_delta : nat;
+    odac_ideal_valid :
+      multicore_semantic_validity jobs m odac_ideal_schedule;
+    odac_default_sources_covered :
+      forall t src,
+        In src
+           (default_event_delay_sources
+              (lex_event
+                 (concrete_to_labeled_execution (oac_execution odac_base)) t)) ->
+        In src (odac_delay_sources t);
+    odac_budget_within_delta :
+      forall t,
+        delay_budget_le
+          odac_delay_bounds
+          odac_delay_sources
+          0
+          t
+          odac_delta;
+    odac_service_lag :
+      service_lag_le
+        m
+        odac_ideal_schedule
+        (labeled_actual_schedule
+           (concrete_to_labeled_execution (oac_execution odac_base)))
+        odac_delta;
+  }.
+
+Record os_delay_top_m_adapter_contract
+    {CState : Type}
+    (P : OSLabeledProjection CState)
+    (spec : GenericTopMSchedulingAlgorithm)
+    (candidates_of : CandidateSource)
+    (jobs : JobId -> Job)
+    (adm : admissible_cpu)
+    (m : nat) : Type :=
+  mkOSDelayTopMAdapterContract {
+    odtac_base : os_multicore_adapter_contract P jobs adm m;
+    odtac_ideal_schedule : Schedule;
+    odtac_delay_bounds : op_delay_bounds;
+    odtac_delay_sources : DelayTrace;
+    odtac_delta : nat;
+    odtac_ideal_top_m :
+      scheduler_rel
+        (top_m_algorithm_schedule spec candidates_of)
+        jobs m odtac_ideal_schedule;
+    odtac_default_sources_covered :
+      forall t src,
+        In src
+           (default_event_delay_sources
+              (lex_event
+                 (concrete_to_labeled_execution (oac_execution odtac_base)) t)) ->
+        In src (odtac_delay_sources t);
+    odtac_budget_within_delta :
+      forall t,
+        delay_budget_le
+          odtac_delay_bounds
+          odtac_delay_sources
+          0
+          t
+          odtac_delta;
+    odtac_service_lag :
+      service_lag_le
+        m
+        odtac_ideal_schedule
+        (labeled_actual_schedule
+           (concrete_to_labeled_execution (oac_execution odtac_base)))
+        odtac_delta;
+  }.
+
+Arguments odac_base {CState P jobs adm m} _.
+Arguments odac_ideal_schedule {CState P jobs adm m} _.
+Arguments odac_delay_bounds {CState P jobs adm m} _.
+Arguments odac_delay_sources {CState P jobs adm m} _ _.
+Arguments odac_delta {CState P jobs adm m} _.
+Arguments odac_ideal_valid {CState P jobs adm m} _.
+Arguments odtac_base {CState P spec candidates_of jobs adm m} _.
+Arguments odtac_ideal_schedule {CState P spec candidates_of jobs adm m} _.
+Arguments odtac_delay_bounds {CState P spec candidates_of jobs adm m} _.
+Arguments odtac_delay_sources {CState P spec candidates_of jobs adm m} _ _.
+Arguments odtac_delta {CState P spec candidates_of jobs adm m} _.
+Arguments odtac_ideal_top_m {CState P spec candidates_of jobs adm m} _.
+
+Lemma os_multicore_adapter_contract_implies_valid_schedule :
+  forall CState (P : OSLabeledProjection CState) jobs adm m
+         (C : os_multicore_adapter_contract P jobs adm m),
+    valid_schedule
+      jobs
+      m
+      (project_schedule
+         (lex_trace (concrete_to_labeled_execution (oac_execution C)))).
+Proof.
+  intros CState P jobs adm m [ex Hsound].
+  apply labeled_concrete_multicore_projection_sound_implies_valid_schedule
+    with (adm := adm).
+  exact Hsound.
+Qed.
+
+Lemma os_multicore_adapter_contract_implies_semantic_validity :
+  forall CState (P : OSLabeledProjection CState) jobs adm m
+         (C : os_multicore_adapter_contract P jobs adm m),
+    multicore_semantic_validity
+      jobs
+      m
+      (project_schedule
+         (lex_trace (concrete_to_labeled_execution (oac_execution C)))).
+Proof.
+  intros CState P jobs adm m [ex Hsound].
+  apply labeled_concrete_multicore_projection_sound_implies_semantic_validity
+    with (adm := adm).
+  exact Hsound.
+Qed.
+
+Lemma os_multicore_adapter_contract_implies_placement :
+  forall CState (P : OSLabeledProjection CState) jobs adm m
+         (C : os_multicore_adapter_contract P jobs adm m),
+    schedule_respects_admissibility
+      adm
+      m
+      (project_schedule
+         (lex_trace (concrete_to_labeled_execution (oac_execution C)))).
+Proof.
+  intros CState P jobs adm m [ex Hsound].
+  apply labeled_concrete_multicore_projection_sound_implies_placement
+    with (jobs := jobs).
+  exact Hsound.
+Qed.
+
+Lemma os_delay_adapter_contract_implies_bounded_delay_refinement :
+  forall CState (P : OSLabeledProjection CState) jobs adm m
+         (C : os_delay_adapter_contract P jobs adm m),
+    let ex := @oac_execution CState P jobs adm m (odac_base C) in
+    bounded_delay_projection_refinement
+      jobs
+      adm
+      m
+      (concrete_to_labeled_execution ex)
+      (odac_ideal_schedule C)
+      (odac_delay_bounds C)
+      (odac_delay_sources C)
+      (odac_delta C).
+Proof.
+  intros CState P jobs adm m C.
+  destruct C as [base ideal bounds sources delta Hvalid Hcovered Hbudget Hlag].
+  destruct base as [ex Hsound].
+  apply mk_bounded_delay_projection_refinement.
+  - apply labeled_concrete_multicore_projection_sound_to_labeled_execution.
+    exact Hsound.
+  - exact Hvalid.
+  - exact Hcovered.
+  - exact Hbudget.
+  - exact Hlag.
+Qed.
+
+Lemma os_delay_top_m_adapter_contract_implies_bounded_delay_top_m_refinement :
+  forall CState (P : OSLabeledProjection CState)
+         spec candidates_of jobs adm m
+         (C : os_delay_top_m_adapter_contract P spec candidates_of jobs adm m),
+    let ex := @oac_execution CState P jobs adm m (odtac_base C) in
+    bounded_delay_top_m_projection_refinement
+      spec
+      candidates_of
+      jobs
+      adm
+      m
+      (concrete_to_labeled_execution ex)
+      (odtac_ideal_schedule C)
+      (odtac_delay_bounds C)
+      (odtac_delay_sources C)
+      (odtac_delta C).
+Proof.
+  intros CState P spec candidates_of jobs adm m C.
+  destruct C as [base ideal bounds sources delta Htopm Hcovered Hbudget Hlag].
+  destruct base as [ex Hsound].
+  apply mk_bounded_delay_top_m_projection_refinement.
+  - apply labeled_concrete_multicore_projection_sound_to_labeled_execution.
+    exact Hsound.
+  - exact Htopm.
+  - exact Hcovered.
+  - exact Hbudget.
+  - exact Hlag.
+Qed.
